TypeSafety.v
@@ -42,19 +42,6 @@ Proof.
     destruct (PeanoNat.Nat.eq_dec _ _); discriminate || eauto.
 Qed.
 
-Definition log_write_consistent (log: Log) (v: fenv nat nat) :=
-  forall reg lvl val n,
-    v reg n ->
-    List.In {| kind := LogWrite; level := lvl; reg := reg; val := val |} log ->
-    n = List.length val.
-
-Definition correct_type `{Env nat bits} v (r: result (Log * value)) (tau: type) :=
-  match r with
-  | Success (l, val) => log_write_consistent l v /\ type_of_value val = tau
-  | CannotRun => True
-  | Stuck => False
-  end.
-
 Ltac not_stuck :=
   intros; unfold may_write, may_read0, may_read1;
   repeat match goal with
@@ -86,13 +73,6 @@ Lemma type_of_value_le_eq:
 Proof.
   destruct v; cbn; inversion 1; congruence.
 Qed.
-
-Axiom get_put_Some: (forall {K V} `{Env K V} ev k k' v v',
-                         getenv (putenv ev k v) k' = Some v' ->
-                         k = k' /\ v = v' \/ k <> k' /\ getenv ev k' = Some v').
-Axiom get_put_None: (forall {K V} `{Env K V} ev k k' v,
-                         getenv (putenv ev k v) k' = None ->
-                         k <> k' /\ getenv ev k' = None).
 
 Section EnvEquiv.
   Context {K V V': Type} {Env: Env K V}.
@@ -130,143 +110,51 @@ Section EnvEquiv.
       getenv gamma k = None ->
       forall v', Gamma k v' -> False.
   Proof. firstorder. Qed.
+
+  Definition tenv_of_env (ev: env_t Env): fenv K V'.
+    refine {| fn k v' := exists v, getenv ev k = Some v /\ v' = f v |}.
+    abstract (intros * (? & Heq & Hfeq) (? & Heq' & Hfeq'); subst;
+              rewrite Heq in Heq'; inversion Heq'; eauto).
+  Defined.
+
+  Lemma tenv_of_env_equiv :
+    forall (ev: env_t Env),
+      env_equiv (tenv_of_env ev) ev.
+  Proof.
+    intros; unfold env_equiv, tenv_of_env, not; cbn; split.
+    - firstorder.
+    - intros * Heq * Hex; rewrite Heq in Hex;
+        firstorder discriminate.
+  Qed.
+
+  Lemma tenv_of_env_nil :
+    env_equiv fenv_nil env_nil.
+    unfold env_equiv, fenv_nil; cbn; split; intros.
+    - rewrite getenv_nil in H; discriminate.
+    - tauto.
+  Qed.
 End EnvEquiv.
 
-(*   Definition gamma_well_typed (Gamma: fenv TVar type) (gamma: env_t GammaEnv) := *)
-(*     (forall var v, getenv gamma var = Some v -> Gamma var (type_of_value v)) /\ *)
-(*     (forall var, getenv gamma var = None -> forall tau, not (Gamma var tau)). *)
-
-
-(* Lemma gamma_well_typed_putenv: *)
-(*   forall (Gamma: fenv TVar type) (gamma: env_t GammaEnv) *)
-(*     (var: TVar) (tau: type) (v: value), *)
-(*     gamma_well_typed Gamma gamma -> *)
-(*     type_of_value v = tau -> *)
-(*     gamma_well_typed (fenv_add Gamma var tau) (putenv gamma var v). *)
-(* Proof. *)
-(*   unfold gamma_well_typed; cbn. intros * (H & H') **. *)
-(*   split; intros; [ *)
-(*     pose proof (get_put_Some _ _ _ _ _ ltac:(eassumption)) | *)
-(*     pose proof (get_put_None _ _ _ _ ltac:(eassumption)) *)
-(*   ]; firstorder (subst; eauto). *)
-(* Qed. *)
-
-(* Lemma gamma_well_typed_getenv_Some: *)
-(*   forall (Gamma: fenv TVar type) (var: TVar) (gamma: env_t GammaEnv), *)
-(*     gamma_well_typed Gamma gamma -> *)
-(*     forall a: value, *)
-(*       getenv gamma var = Some a -> *)
-(*       Gamma var (type_of_value a). *)
-(* Proof. firstorder. Qed. *)
-
-(* Lemma gamma_well_typed_getenv_None: *)
-(*   forall (Gamma: fenv TVar type) (var: TVar) (gamma: env_t GammaEnv), *)
-(*     gamma_well_typed Gamma gamma -> *)
-(*     getenv gamma var = None -> *)
-(*     forall tau, *)
-(*       Gamma var tau -> False. *)
-(* Proof. firstorder. Qed. *)
-
-Ltac constr_hd c :=
-      match c with
-      | ?f ?x => constr_hd f
-      | ?g => g
-      end.
-
-Section TypeSafety.
-  Context {TVar: Type}.
-  Context {TFn: Type}.
-
-  Context (GammaEnv: Env TVar value).
-  Context (SigmaEnv: Env TFn ExternalFunction).
-  Context (RegEnv: Env nat bits).
-
-  Hint Resolve (@env_equiv_putenv _ _ _ GammaEnv): types.
-
-Definition and_fst {A B} := fun '(conj a _: and A B) => a.
-Definition and_snd {A B} := fun '(conj _ b: and A B) => b.
-
-Ltac t_step :=
-  match goal with
-  | _ => discriminate
-  | _ => progress (cbn in *; intros; subst)
-  | [  |- _ /\ _ ] => split
-  | [ H: _ /\ _ |- _ ] => destruct H
-  | [ H: Success _ = Success _ |- _ ] =>
-    inversion H; clear H
-  | [ H: bit_t _ = bit_t _ |- _ ] =>
-    inversion H; clear H
-  | [ H: ExternalFunction |- _ ] => destruct H
-  | [ H: ?a, H': ?a |- _ ] =>
-    let ta := type of a in
-    unify ta Prop; clear H'
-  | [ H: log_find _ _ _ = Some _ |- _ ] =>
-    unfold log_find in H; apply List.find_some in H
-  | [ H: List.In ?x (?a ++ ?b) |- _ ] =>
-    pose_once (List.in_app_or a b x) H
-  | [ H: forall _, env_equiv _ ?Gamma _ -> _,
-        H': env_equiv _ ?Gamma _ |- _ ] =>
-    specialize (H _ H')
-  | [ H: @fn ?K ?V ?ev ?k ?v, H': fn ?ev ?k ?v' |- _ ] =>
-    pose_once (@uniq K V ev k v v') H H'
-  | [ H: _ |- _ ] => apply forall2_fold_right2 in H
-  | [ H: @log_write_consistent ?log ?v,
-         H': fn ?v ?reg ?val,
-             H'': In {| kind := LogWrite; reg := ?reg; level := ?lvl; val := ?val' |} ?log |- _ ] =>
-    pose_once (H reg lvl val' val) H' H''
-  | [ H: forall log, log_write_consistent log _ -> correct_type _ (interp _ _ _ _ log _) _,
-      H': log_write_consistent ?log _ |- _ ] =>
-    pose_once H log H'
-  | [ H: env_equiv (Env := ?Env) ?f ?tenv ?env,
-      H': getenv ?env ?k = Some ?v |- _ ] =>
-    pose_once (and_fst H k v) H'
-  | [ H: env_equiv ?f ?tenv ?env,
-         H': getenv ?env ?k = None |- _ ] =>
-    pose_once (and_snd H k) H'
-  | [ H: assert_size _ _ = Success _ |- _ ] =>
-    apply assert_size_Success in H
-  | [ H: assert_size _ _ = Stuck |- _ ] =>
-    apply assert_size_Stuck in H
-  | [ H: opt_result Stuck _ = Success _ |- _ ] =>
-    apply opt_result_Success in H
-  | [ H: opt_result Stuck _ = Stuck |- _ ] =>
-    apply opt_result_Stuck in H
-  | [ p: _ * _ |- _ ] => destruct p
-  | [  |- _ (opt_result _ ?o) _] =>
-    destruct o eqn:?
-  | [  |- correct_type _ (result_bind ?r _) _ ] =>
-    destruct r eqn:?
-  | [  |- correct_type _ (result_map ?r _) _ ] =>
-    destruct r eqn:?
-  | [  |- correct_type _ ((if ?v then _ else _)) _ ] =>
-    destruct v eqn:?
-  | [ H: correct_type _ (interp _ ?Gamma _ _ ?log ?s) _,
-         H': interp _ ?Gamma _ _ ?log ?s = Stuck |- _ ] =>
-    red in H; rewrite H' in H
-  | [ H: match ?x with _ => _ end = ?c |- _ ] =>
-    let c_hd := constr_hd c in
-    is_constructor c_hd; destruct x
-  | [ H: _ \/ _ |- _ ] => destruct H
-  | _ => progress (unfold assert_bits, may_read1 in *)
-  | _ => solve [eauto 4 using eq_trans with types]
-  end.
-
-Ltac t :=
-  repeat t_step;
-  repeat match goal with
-         | [ H: Posed _ |- _ ] => clear H
-         end.
-
-Definition tenv_of_env {K V V'} {env: Env K V} {f: V -> V'} (ev: env_t env): fenv K V'.
-  refine {| fn k v' := exists v, getenv ev k = Some v /\ v' = f v |}.
-  abstract (intros * (? & Heq & Hfeq) (? & Heq' & Hfeq'); subst;
-            rewrite Heq in Heq'; inversion Heq'; eauto).
-Defined.
+Definition log_write_consistent (log: Log) (v: fenv nat nat) :=
+  forall reg lvl val n,
+    v reg n ->
+    List.In {| kind := LogWrite; level := lvl; reg := reg; val := val |} log ->
+    n = List.length val.
 
 Lemma log_write_consistent_nil:
   forall v, log_write_consistent nil v.
 Proof.
   unfold log_write_consistent; cbn; tauto.
+Qed.
+
+Lemma log_write_consistent_app:
+  forall (v: fenv nat nat) (sched_log rule_log: Log),
+    log_write_consistent sched_log v ->
+    log_write_consistent rule_log v ->
+    log_write_consistent (rule_log ++ sched_log) v.
+Proof.
+  unfold log_write_consistent; simpl; intros * Hsched Hrul * Hsize Hin.
+  apply in_app_or in Hin; firstorder.
 Qed.
 
 Lemma log_read_consistent_add:
@@ -295,155 +183,270 @@ Qed.
 
 Hint Resolve log_write_consistent_add: types.
 
-Lemma type_safe_call:
-  forall v V sigma Sigma gamma Gamma,
-    env_equiv (@length bool) v V ->
-    env_equiv sig sigma Sigma ->
-    forall sched_log retType args sizes impl,
-      length args = length sizes ->
-      env_equiv type_of_value gamma Gamma ->
-      (forall args : list bits,
-          length args = length sizes ->
-          type_of_value (impl args) = retType) ->
-      (fold_right2
-         (fun arg argSize acc =>
-            acc /\
-            (forall Gamma : env_t GammaEnv,
-                env_equiv type_of_value gamma Gamma ->
-                forall rule_log : Log,
-                  log_write_consistent rule_log v ->
-                  correct_type v (interp V Sigma Gamma sched_log rule_log arg) (bit_t argSize))) True args sizes) ->
-      (fold_right2
-         (fun arg argSize acc =>
-            acc /\ HasType v sigma gamma arg (bit_t argSize)) True args sizes) ->
-      forall (rule_log: Log),
-        log_write_consistent rule_log v ->
-        forall argvs0 res,
-          fold_left2
-            (fun (acc: result (Log * list bits)) arg size =>
-               result_bind acc (fun '(rule_log, argvs) =>
-               result_bind (interp V Sigma Gamma sched_log rule_log arg) (fun '(rule_log, argv) =>
-               result_map (assert_bits argv size) (fun bs =>
-               (rule_log, bs :: argvs)))))
-            args sizes (Success (rule_log, argvs0)) = res ->
-          res = CannotRun \/
-          exists argvs rule_log',
-            res = Success (rule_log', argvs ++ argvs0) /\
-            length argvs = length sizes /\
-            log_write_consistent rule_log' v /\
-            type_of_value (impl argvs) = retType.
-Proof.
-  induction args; destruct sizes; inversion 1.
-  - cbn. intros **; destruct res; try discriminate.
-    inversion H7; subst; right; exists nil; eexists; intuition eauto.
-  - cbn in *; intros Heqv Htypeof (Hargscorrect & Hargcorrect) (Hargtypes & Hargtype) * Hconsistent * Heq.
-    specialize (Hargcorrect _ ltac:(eassumption) _ ltac:(eassumption)).
-    destruct interp as [(? & ?) | | ] eqn:?; cbn in *; try tauto.
-    + destruct Hargcorrect as (Hlconsistent & Htypev0).
-      destruct v0; cbn in *; try discriminate.
-      inversion Htypev0; subst n; clear Htypev0.
-      unfold assert_size in *.
-      destruct PeanoNat.Nat.eq_dec; try congruence; cbn in *.
+Section TypeSafety.
+  Context {TVar: Type}.
+  Context {TFn: Type}.
 
-      specialize (IHargs sizes (fun args => impl (args ++ [val]))
-                         ltac:(eassumption) ltac:(eassumption)).
-      specialize (IHargs ltac:(intros; apply Htypeof; rewrite app_length, PeanoNat.Nat.add_comm; cbn; eauto)
-                         ltac:(eassumption) ltac:(eassumption)
-                                                   l ltac:(eassumption) _ _ Heq).
-      destruct IHargs as [ IHargs | IHargs ]; [ now left | right ].
-      destruct IHargs as (argvs & rule_log' & Hreseq & Hlen & Hconsistent' & Htypeof'); subst.
-      exists (argvs ++ [val]); exists rule_log'.
-      repeat split.
-      * rewrite <- app_assoc; reflexivity.
-      * rewrite app_length, PeanoNat.Nat.add_comm; cbn; eauto.
-      * eauto.
-    + (* rewrite fold_left2_rev_right2 in Heq by assumption. *)
-      clear -Heq.
-      left; revert dependent sizes; induction args; destruct sizes; cbn in *; eauto.
-Qed.
+  Context (GammaEnv: Env TVar value).
+  Context (SigmaEnv: Env TFn ExternalFunction).
+  Context (RegEnv: Env nat bits).
 
-Lemma type_safety'':
-  forall sigma Sigma gamma v V sched_log,
-    env_equiv (@length bool) v V ->
-    env_equiv sig sigma Sigma ->
-    log_write_consistent sched_log v ->
-    forall (s: syntax TVar TFn)
-      (tau: Types.type),
-      Typechecking.HasType v sigma gamma s tau ->
-      forall Gamma,
+  Hint Resolve (@env_equiv_putenv _ _ _ GammaEnv): types.
+
+  Definition correct_type `{Env nat bits} v (r: result (Log * value)) (tau: type) :=
+    match r with
+    | Success (l, val) => log_write_consistent l v /\ type_of_value val = tau
+    | CannotRun => True
+    | Stuck => False
+    end.
+
+  Ltac t_step :=
+    match goal with
+    | _ => discriminate
+    | _ => progress (cbn in *; intros; subst)
+    | [  |- _ /\ _ ] => split
+    | [ H: _ /\ _ |- _ ] => destruct H
+    | [ H: Success _ = Success _ |- _ ] =>
+      inversion H; clear H
+    | [ H: bit_t _ = bit_t _ |- _ ] =>
+      inversion H; clear H
+    | [ H: ExternalFunction |- _ ] => destruct H
+    | [ H: ?a, H': ?a |- _ ] =>
+      let ta := type of a in
+      unify ta Prop; clear H'
+    | [ H: log_find _ _ _ = Some _ |- _ ] =>
+      unfold log_find in H; apply List.find_some in H
+    | [ H: List.In ?x (?a ++ ?b) |- _ ] =>
+      pose_once (List.in_app_or a b x) H
+    | [ H: forall _, env_equiv _ ?Gamma _ -> _,
+          H': env_equiv _ ?Gamma _ |- _ ] =>
+      specialize (H _ H')
+    | [ H: @fn ?K ?V ?ev ?k ?v, H': fn ?ev ?k ?v' |- _ ] =>
+      pose_once (@uniq K V ev k v v') H H'
+    | [ H: _ |- _ ] => apply forall2_fold_right2 in H
+    | [ H: @log_write_consistent ?log ?v,
+           H': fn ?v ?reg ?val,
+               H'': In {| kind := LogWrite; reg := ?reg; level := ?lvl; val := ?val' |} ?log |- _ ] =>
+      pose_once (H reg lvl val' val) H' H''
+    | [ H: forall log, log_write_consistent log _ -> correct_type _ (interp_rule _ _ _ _ log _) _,
+        H': log_write_consistent ?log _ |- _ ] =>
+      pose_once H log H'
+    | [ H: env_equiv (Env := ?Env) ?f ?tenv ?env,
+        H': getenv ?env ?k = Some ?v |- _ ] =>
+      pose_once (and_fst H k v) H'
+    | [ H: env_equiv ?f ?tenv ?env,
+           H': getenv ?env ?k = None |- _ ] =>
+      pose_once (and_snd H k) H'
+    | [ H: assert_size _ _ = Success _ |- _ ] =>
+      apply assert_size_Success in H
+    | [ H: assert_size _ _ = Stuck |- _ ] =>
+      apply assert_size_Stuck in H
+    | [ H: opt_result Stuck _ = Success _ |- _ ] =>
+      apply opt_result_Success in H
+    | [ H: opt_result Stuck _ = Stuck |- _ ] =>
+      apply opt_result_Stuck in H
+    | [ p: _ * _ |- _ ] => destruct p
+    | [  |- _ (opt_result _ ?o) _] =>
+      destruct o eqn:?
+    | [  |- correct_type _ (result_bind ?r _) _ ] =>
+      destruct r eqn:?
+    | [  |- correct_type _ (result_map ?r _) _ ] =>
+      destruct r eqn:?
+    | [  |- correct_type _ ((if ?v then _ else _)) _ ] =>
+      destruct v eqn:?
+    | [ H: correct_type _ (interp_rule _ ?Gamma _ _ ?log ?s) _,
+           H': interp_rule _ ?Gamma _ _ ?log ?s = Stuck |- _ ] =>
+      red in H; rewrite H' in H
+    | [ H: match ?x with _ => _ end = ?c |- _ ] =>
+      let c_hd := constr_hd c in
+      is_constructor c_hd; destruct x
+    | [ H: _ \/ _ |- _ ] => destruct H
+    | _ => progress (unfold assert_bits, may_read1 in *)
+    | _ => solve [eauto 4 using eq_trans with types]
+    end.
+
+  Ltac t :=
+    repeat t_step;
+    repeat match goal with
+           | [ H: Posed _ |- _ ] => clear H
+           end.
+
+  Lemma type_safe_call:
+    forall v V sigma Sigma gamma Gamma,
+      env_equiv (@length bool) v V ->
+      env_equiv sig sigma Sigma ->
+      forall sched_log retType args sizes impl,
+        length args = length sizes ->
         env_equiv type_of_value gamma Gamma ->
-        forall rule_log: Log,
+        (forall args : list bits,
+            length args = length sizes ->
+            type_of_value (impl args) = retType) ->
+        (fold_right2
+           (fun arg argSize acc =>
+              acc /\
+              (forall Gamma : env_t GammaEnv,
+                  env_equiv type_of_value gamma Gamma ->
+                  forall rule_log : Log,
+                    log_write_consistent rule_log v ->
+                    correct_type v (interp_rule V Sigma Gamma sched_log rule_log arg) (bit_t argSize))) True args sizes) ->
+        (fold_right2
+           (fun arg argSize acc =>
+              acc /\ HasType v sigma gamma arg (bit_t argSize)) True args sizes) ->
+        forall (rule_log: Log),
           log_write_consistent rule_log v ->
-          correct_type v (interp V Sigma Gamma sched_log rule_log s) tau.
-Proof.
-  induction 4; cbn; intros.
+          forall argvs0 res,
+            fold_left2
+              (fun (acc: result (Log * list bits)) arg size =>
+                 result_bind acc (fun '(rule_log, argvs) =>
+                 result_bind (interp_rule V Sigma Gamma sched_log rule_log arg) (fun '(rule_log, argv) =>
+                 result_map (assert_bits argv size) (fun bs =>
+                 (rule_log, bs :: argvs)))))
+              args sizes (Success (rule_log, argvs0)) = res ->
+            res = CannotRun \/
+            exists argvs rule_log',
+              res = Success (rule_log', argvs ++ argvs0) /\
+              length argvs = length sizes /\
+              log_write_consistent rule_log' v /\
+              type_of_value (impl argvs) = retType.
+  Proof.
+    induction args; destruct sizes; inversion 1.
+    - cbn. intros **; destruct res; try discriminate.
+      inversion H7; subst; right; exists nil; eexists; intuition eauto.
+    - cbn in *; intros Heqv Htypeof (Hargscorrect & Hargcorrect) (Hargtypes & Hargtype) * Hconsistent * Heq.
+      specialize (Hargcorrect _ ltac:(eassumption) _ ltac:(eassumption)).
+      destruct interp_rule as [(? & ?) | | ] eqn:?; cbn in *; try tauto.
+      + destruct Hargcorrect as (Hlconsistent & Htypev0).
+        destruct v0; cbn in *; try discriminate.
+        inversion Htypev0; subst n; clear Htypev0.
+        unfold assert_size in *.
+        destruct PeanoNat.Nat.eq_dec; try congruence; cbn in *.
 
-  all: try solve [t].
+        specialize (IHargs sizes (fun args => impl (args ++ [val]))
+                           ltac:(eassumption) ltac:(eassumption)).
+        specialize (IHargs ltac:(intros; apply Htypeof; rewrite app_length, PeanoNat.Nat.add_comm; cbn; eauto)
+                           ltac:(eassumption) ltac:(eassumption)
+                                                     l ltac:(eassumption) _ _ Heq).
+        destruct IHargs as [ IHargs | IHargs ]; [ now left | right ].
+        destruct IHargs as (argvs & rule_log' & Hreseq & Hlen & Hconsistent' & Htypeof'); subst.
+        exists (argvs ++ [val]); exists rule_log'.
+        repeat split.
+        * rewrite <- app_assoc; reflexivity.
+        * rewrite app_length, PeanoNat.Nat.add_comm; cbn; eauto.
+        * eauto.
+      + (* rewrite fold_left2_rev_right2 in Heq by assumption. *)
+        clear -Heq.
+        left; revert dependent sizes; induction args; destruct sizes; cbn in *; eauto.
+  Qed.
 
-  - t;
-      destruct (interp V Sigma Gamma0 sched_log rule_log s) as [ (? & ?) | | ]; cbn in *;
-        firstorder eauto using type_of_value_le_eq.
+  Lemma rule_safety'':
+    forall sigma Sigma gamma v V sched_log,
+      env_equiv (@length bool) v V ->
+      env_equiv sig sigma Sigma ->
+      log_write_consistent sched_log v ->
+      forall (s: rule TVar TFn)
+        (tau: Types.type),
+        HasType v sigma gamma s tau ->
+        forall Gamma,
+          env_equiv type_of_value gamma Gamma ->
+          forall rule_log: Log,
+            log_write_consistent rule_log v ->
+            correct_type v (interp_rule V Sigma Gamma sched_log rule_log s) tau.
+  Proof.
+    induction 4; cbn; intros.
 
-  - t.
+    all: try solve [t].
 
-    all: eapply type_safe_call in Heqr0; eauto using type_ok.
-    all: repeat match goal with
-                | [ H: exists _, _ |- _ ] => destruct H
-                | [  |- context[_ ++ nil] ] => rewrite app_nil_r
-                | _ => t_step
-                end.
-Qed.
+    - t;
+        destruct (interp_rule V Sigma Gamma0 sched_log rule_log s) as [ (? & ?) | | ]; cbn in *;
+          firstorder eauto using type_of_value_le_eq.
 
-Lemma type_safety':
-  forall sigma Sigma gamma Gamma v V sched_log rule_log,
-    env_equiv sig sigma Sigma ->
-    env_equiv (@length bool) v V ->
-    env_equiv type_of_value gamma Gamma ->
-    log_write_consistent sched_log v ->
-    log_write_consistent rule_log v ->
-    forall s tau,
-      Typechecking.HasType v sigma gamma s tau ->
-      interp V Sigma Gamma sched_log rule_log s <> CannotRun ->
-      exists rule_log' val,
-        interp V Sigma Gamma sched_log rule_log s = Success (rule_log', val) /\
-        log_write_consistent rule_log' v /\
-        type_of_value val = tau.
-Proof.
-  intros;
-    pose proof (type_safety'' sigma Sigma gamma v V sched_log) as ts;
-    repeat specialize (ts ltac:(eassumption));
-    unfold correct_type in ts.
-  destruct interp as [(? & ?) | | ]; cbn in *; (congruence || tauto || eauto).
-Qed.
+    - t.
 
-Lemma tenv_of_env_equiv  {K V V'} {env: Env K V} {f: V -> V'} :
-  forall (ev: env_t env),
-    env_equiv f (tenv_of_env (f := f) ev) ev.
-Proof.
-  intros; unfold env_equiv, tenv_of_env, not; cbn; split.
-  - firstorder.
-  - intros * Heq * Hex; rewrite Heq in Hex;
-      firstorder discriminate.
-Qed.
+      all: eapply type_safe_call in Heqr0; eauto using type_ok.
+      all: repeat match goal with
+                  | [ H: exists _, _ |- _ ] => destruct H
+                  | [  |- context[_ ++ nil] ] => rewrite app_nil_r
+                  | _ => t_step
+                  end.
+  Qed.
 
-Theorem type_safety:
-  forall Sigma Gamma V sched_log,
-    let sigma := tenv_of_env (f := sig) Sigma in
-    let v := tenv_of_env (f := (@length bool)) V in
-    let gamma := tenv_of_env (f := type_of_value) Gamma in
-    log_write_consistent sched_log v ->
-    forall s tau,
-      Typechecking.HasType v sigma gamma s tau ->
-      interp V Sigma Gamma sched_log [] s = CannotRun \/
-      exists rule_log' val,
-        interp V Sigma Gamma sched_log [] s = Success (rule_log', val) /\
-        log_write_consistent rule_log' v /\
-        type_of_value val = tau.
-Proof.
-  cbv zeta; intros.
-  destruct interp eqn:Heq; [right | eauto | right];
-    rewrite <- Heq;
-    eapply type_safety';
-    try eapply tenv_of_env_equiv.
-  all: revgoals; eauto using log_write_consistent_nil || congruence.
-Qed.
+  Lemma rule_safety':
+    forall sigma Sigma gamma Gamma v V sched_log rule_log,
+      env_equiv sig sigma Sigma ->
+      env_equiv (@length bool) v V ->
+      env_equiv type_of_value gamma Gamma ->
+      log_write_consistent sched_log v ->
+      log_write_consistent rule_log v ->
+      forall s tau,
+        HasType v sigma gamma s tau ->
+        interp_rule V Sigma Gamma sched_log rule_log s <> CannotRun ->
+        exists rule_log' val,
+          interp_rule V Sigma Gamma sched_log rule_log s = Success (rule_log', val) /\
+          log_write_consistent rule_log' v /\
+          type_of_value val = tau.
+  Proof.
+    intros;
+      pose proof (rule_safety'' sigma Sigma gamma v V sched_log) as ts;
+      repeat specialize (ts ltac:(eassumption));
+      unfold correct_type in ts.
+    destruct interp_rule as [(? & ?) | | ]; cbn in *; (congruence || tauto || eauto).
+  Qed.
+
+  Theorem rule_safety:
+    forall Sigma V sched_log,
+      let sigma := tenv_of_env sig Sigma in
+      let v := tenv_of_env ((@length bool)) V in
+      log_write_consistent sched_log v ->
+      forall s tau,
+        HasType v sigma fenv_nil s tau ->
+        interp_rule V Sigma env_nil sched_log [] s = CannotRun \/
+        exists rule_log' val,
+          interp_rule V Sigma env_nil sched_log [] s = Success (rule_log', val) /\
+          log_write_consistent rule_log' v /\
+          type_of_value val = tau.
+  Proof.
+    cbv zeta; intros.
+    destruct interp_rule eqn:Heq; [right | eauto | right];
+      rewrite <- Heq;
+      eapply rule_safety';
+      try eapply tenv_of_env_nil;
+      try eapply tenv_of_env_equiv.
+    all: revgoals; eauto using log_write_consistent_nil || congruence.
+  Qed.
+
+  Lemma scheduler_safety':
+    forall Sigma V s sigma v,
+      SchedulerHasTypes v sigma s ->
+      forall sched_log,
+        env_equiv sig sigma Sigma ->
+        env_equiv (@length bool) v V ->
+        log_write_consistent sched_log v ->
+        exists sched_log',
+          interp_scheduler V Sigma sched_log s = Some sched_log' /\
+          log_write_consistent sched_log' v.
+  Proof.
+    induction 1; cbn.
+    - eauto.
+    - intros.
+      pose proof (rule_safety' sigma Sigma fenv_nil env_nil v V sched_log nil) as rs.
+      repeat (specialize (rs ltac:(eapply tenv_of_env_nil || eauto using log_write_consistent_nil))).
+      destruct interp_rule;
+        try (specialize (rs ltac:(intro; discriminate));
+             destruct rs as (? & ? & Hrw & ? & ?);
+             inversion Hrw; subst); eauto using log_write_consistent_app.
+  Qed.
+
+  Lemma scheduler_safety:
+    forall s Sigma V sched_log,
+      let sigma := tenv_of_env sig Sigma in
+      let v := tenv_of_env ((@length bool)) V in
+      log_write_consistent sched_log v ->
+      SchedulerHasTypes v sigma s ->
+      exists sched_log',
+        interp_scheduler V Sigma sched_log s = Some sched_log' /\
+        log_write_consistent sched_log' v.
+  Proof.
+    cbv zeta; intros; eapply scheduler_safety';
+      try eapply tenv_of_env_equiv; eauto.
+  Qed.
+End TypeSafety.
